Mostly verifying, now we need the special sauce

Source/DafnyRuntime/dafnySequence.dfy
@@ -7,36 +7,7 @@ module {:options "/functionSyntax:4"} MetaSeq {
 
   import opened Stacks
 
-  trait Seq<T> {
-    predicate Valid()
-
-    method Length() returns (l: nat)
-
-    function At(i: nat): T
-
-    method Concatenate(s: Seq<T>) returns (l: Seq<T>)
-
-    method Slice(start: nat, end: nat) returns (s: Seq<T>)
-      requires start <= end <= Length()
-  }
-
-  class ArraySeq<T> extends Seq<T> {
-    const values: array<T>
-
-    constructor(s: seq<T>) {
-
-    }
-  }
-
-  class ConcatSeq<T> extends Seq<T> {
-    
-  }
-
-  class LazySeq<T> extends Seq<T> {
-    var 
-  }
-
-  datatype Seq<T> = Empty | Direct(a: seq<T>) | Concat(left: Seq<T>, right: Seq<T>, length: nat) {
+  datatype SeqExpr<T> = Empty | Direct(a: seq<T>) | Concat(left: SeqExpr<T>, right: SeqExpr<T>, length: nat) {
 
     predicate Valid() {
       match this
@@ -58,15 +29,12 @@ module {:options "/functionSyntax:4"} MetaSeq {
       requires Valid()
       requires i < Length()
     {
-      Force()[i]
+      Value()[i]
     }
 
-    function Concatenate(s: Seq<T>): Seq<T> {
+    function Concatenate(s: SeqExpr<T>): SeqExpr<T> {
       Concat(this, s, Length() + s.Length())
     }
-
-    method Slice(start: nat, end: nat) returns (s: Seq<T>)
-      requires start <= end <= Length()
 
     function Value(): seq<T> 
       requires Valid()
@@ -77,24 +45,13 @@ module {:options "/functionSyntax:4"} MetaSeq {
       case Direct(a) => a
       case Concat(left, right, _) => left.Value() + right.Value()
     }
-
-    // TODO: {:memoize} should result in thread-safe lazy evaluation in each runtime
-    function {:memoize} Force(): seq<T> 
-      requires Valid()
-    {
-      Value()
-    } by method {
-      match this
-      case Concat(left, right, length) => return CalcConcat(left, right, length);
-      case _ => return Value();
-    }
   }
 
-  function CalcConcat<T>(left: Seq<T>, right: Seq<T>, length: nat): seq<T> {
+  function CalcConcat<T>(left: SeqExpr<T>, right: SeqExpr<T>, length: nat): seq<T> {
     left.Value() + right.Value()
   } by method {
     var builder: SeqBuilder<T> := new SeqBuilder(length);
-    var toVisit := new Stack<Seq<T>>(Empty);
+    var toVisit := new Stack<SeqExpr<T>>(Empty);
     :- expect toVisit.Push(right);
     :- expect toVisit.Push(left);
 
@@ -139,6 +96,138 @@ module {:options "/functionSyntax:4"} MetaSeq {
 
     function Value(): seq<T> reads this {
       s
+    }
+  }
+
+  trait {:termination false} Validatable {
+    // Ghost state tracking the common set of objects most
+    // methods need to read.
+    ghost var Repr: set<object>
+
+    ghost predicate Valid()
+      reads this, Repr
+      ensures Valid() ==> this in Repr
+
+    // Convenience predicate for when your object's validity depends on one
+    // or more other objects.
+    ghost predicate ValidComponent(component: Validatable)
+      reads this, Repr 
+    {
+      && component in Repr
+      && component.Repr <= Repr
+      && this !in component.Repr
+      && component.Valid()
+    }
+
+    // Convenience predicate, since you often want to assert that 
+    // new objects in Repr are fresh as well in most postconditions.
+    twostate predicate ValidAndDisjoint()
+      reads this, Repr
+    {
+      Valid() && fresh(Repr - old(Repr))
+    }
+  }
+
+  trait Seq<T> extends Validatable {
+    ghost predicate Valid()
+      reads this, Repr
+      ensures Valid() ==> this in Repr
+
+    function Value(): seq<T>
+      requires Valid()
+      reads Repr
+      ensures |Value()| == Length()
+
+    function Length(): nat
+      requires Valid()
+      reads Repr
+
+    function At(i: nat): T
+      reads this, Repr
+      requires Valid()
+      requires i < Length()
+
+    method Concatenate(s: Seq<T>) returns (l: Seq<T>)
+      requires Valid() && s.Valid()
+      ensures l.Valid()
+  }
+
+  // class ArraySeq<T> extends Seq<T> {
+  //   const values: array<T>
+
+  //   constructor(s: seq<T>) {
+  //     values := new T[|s|] (i requires 0 <= i < |s| => s[i]);
+  //   }
+  // }
+
+  class LazySeq<T> extends Seq<T> {
+    var expr: SeqExpr<T>
+
+    constructor(expr: SeqExpr<T>) 
+      requires expr.Valid()
+      ensures Valid()
+    {
+      this.expr := expr;
+      this.Repr := {this};
+    }
+
+    ghost predicate Valid() 
+      reads this, Repr
+      ensures Valid() ==> this in Repr
+    {
+      Repr == {this} && expr.Valid()
+    }
+
+    function Value(): seq<T> 
+      requires Valid()
+      reads Repr
+      ensures |Value()| == Length()
+    {
+      expr.Value()
+    }
+
+    function Length(): nat 
+      requires Valid()
+      reads Repr
+    {
+      expr.Length()
+    }
+
+    method Concatenate(s: Seq<T>) returns (l: Seq<T>) 
+      requires Valid() && s.Valid()
+      ensures l.Valid()
+    {
+      var sLength := s.Length();
+      if (s as Seq<T>) is LazySeq<T> {
+        var lazyS := (s as Seq<T>) as LazySeq<T>;
+        l := new LazySeq(Concat(expr, lazyS.expr, expr.Length() + sLength));
+      } else {
+        l := new LazySeq(Concat(expr, Direct(s.Value()), expr.Length() + sLength));
+      }
+      
+    }
+
+    method Force()
+    {
+      match expr
+      case Concat(left, right, length) => {
+        var s := CalcConcat(left, right, length);
+        expr := Direct(s);
+      }
+      case _ =>
+    }
+
+    function At(i: nat): T 
+      requires Valid()
+      requires i < Length()
+      reads this, Repr
+    {
+      assert expr.Valid();
+      expr.At(i)
+    }
+    by method {
+      Force();
+      return expr.At(i);
     }
   }
 }
